theories/theories/utp_theory.thy
@@ -22,19 +22,25 @@ definition is_healthy ::
 declare is_healthy_def [eval]
 
 definition IDEMPOTENT_OVER ::
-  "'VALUE VAR set \<Rightarrow> 'VALUE WF_FUNCTION set" where
+  "'a VAR set \<Rightarrow> 'a WF_FUNCTION set" where
 "IDEMPOTENT_OVER vs = {f . \<forall> p \<in> WF_PREDICATE_OVER vs . f (f p) = f p}"
 
-definition WF_THEORY :: "('VALUE VAR set set * 'VALUE WF_FUNCTION set) set" where
+type_synonym 'a THEORY = "('a VAR set set * 'a WF_FUNCTION set)"
+
+definition WF_THEORY :: "('a THEORY) set" where
 "WF_THEORY = {(A,H) | A H . \<forall>a\<in>A. \<forall> hc\<in>H. hc \<in> IDEMPOTENT_OVER a}"
 
-typedef 'VALUE WF_THEORY = "WF_THEORY :: (('VALUE VAR) set set * 'VALUE WF_FUNCTION set) set"
+typedef 'a WF_THEORY = "WF_THEORY :: ('a THEORY) set"
   morphisms DestTheory MkTheory
   by (auto simp add:WF_THEORY_def)
 
 declare DestTheory [simp]
 declare DestTheory_inverse [simp]
 declare MkTheory_inverse [simp]
+
+lemma DestTheory_intro [intro]:
+  "(\<And> b. DestTheory x = DestTheory y) \<Longrightarrow> x = y"
+  by (auto simp add: DestTheory_inject[THEN sym])
 
 setup_lifting type_definition_WF_THEORY
 
@@ -48,5 +54,40 @@ definition healthconds ::
 
 definition THEORY_PRED :: "'VALUE WF_THEORY \<Rightarrow> 'VALUE WF_PREDICATE set" where
 "THEORY_PRED t \<equiv> {p. (\<exists> a \<in> \<A> t. UNREST (VAR - a) p) \<and>  (\<forall> H \<in> \<H> t. p is H)}"
+
+instantiation WF_THEORY :: (VALUE) join_semilattice_zero
+begin
+
+lift_definition zero_WF_THEORY :: "'a WF_THEORY" is "(UNIV, {}) :: 'a THEORY"
+  by (simp add:WF_THEORY_def)
+
+lift_definition plus_WF_THEORY :: "'a::VALUE WF_THEORY \<Rightarrow> 'a WF_THEORY \<Rightarrow> 'a WF_THEORY" 
+is "(\<lambda> (A1,HC1) (A2,HC2). (A1\<inter>A2,HC1\<union>HC2)) :: 'a THEORY \<Rightarrow> 'a THEORY \<Rightarrow> 'a THEORY"
+  by (auto simp add:WF_THEORY_def)
+
+definition less_eq_WF_THEORY :: "'a WF_THEORY \<Rightarrow> 'a WF_THEORY \<Rightarrow> bool" where
+"less_eq_WF_THEORY x y \<longleftrightarrow> x + y = y"
+
+definition less_WF_THEORY :: "'a WF_THEORY \<Rightarrow> 'a WF_THEORY \<Rightarrow> bool" where
+"less_WF_THEORY x y \<longleftrightarrow> x \<le> y \<and> x \<noteq> y"
+
+instance
+  apply (intro_classes)
+  apply (simp add:less_eq_WF_THEORY_def)
+  apply (simp add:less_WF_THEORY_def)
+  apply (rule DestTheory_intro)
+  apply (auto simp add:plus_WF_THEORY.rep_eq zero_WF_THEORY.rep_eq)
+  apply (case_tac "DestTheory x", case_tac "DestTheory y", case_tac "DestTheory z")
+  apply (auto)
+  apply (rule DestTheory_intro)
+  apply (auto simp add:plus_WF_THEORY.rep_eq zero_WF_THEORY.rep_eq)
+  apply (case_tac "DestTheory x", case_tac "DestTheory y")
+  apply (auto)
+  apply (rule DestTheory_intro)
+  apply (auto simp add:plus_WF_THEORY.rep_eq zero_WF_THEORY.rep_eq)
+  apply (case_tac "DestTheory x")
+  apply (auto)
+done
+end
 
 end
